Figured out what issue was in tr_to

src/verification/verify.lean
@@ -17,10 +17,11 @@ import data.pfun
 section
 
 parameters (R : Type)
-[add_zero_class R] [has_one R] [has_mul R]
-
-
 open Types (nn rr bb)
+
+section compiler
+
+parameters [add_comm_monoid R] [has_one R] [has_mul R]
 
 @[reducible]
 def ExprVal : Types → Type
@@ -552,7 +553,7 @@ begin
   have := (h ctx).hinit hctx, simp at this,
   obtain ⟨cinit, hc₁, hc₂⟩ := this, 
   have : s.ctx_inv cinit := sorry, -- TODO: Initialize preserves ctx_inv
-  simp [Evalable.eval, (h ctx).hbound, hc₁, hc₂, tr_to.eval_steps_eq h this],
+  simp [StreamExec.eval, Evalable.eval, (h ctx).hbound, hc₁, hc₂, tr_to.eval_steps_eq h this],
 end
 
 end translate
@@ -603,11 +604,16 @@ by { rw bimap_is_defined hx, have := hx.hcurr, simp [imp_iff_distrib], tauto, }
 
 end functor_is_defined
 
-lemma contract_tr [Evalable ι ι'] [Evalable α β] (x : BoundedStreamGen ι α)
+lemma contract_spec [Evalable ι ι'] [Evalable α β] (x : BoundedStreamGen ι α)
   (ctx : EContext) (hctx : x.ctx_inv ctx)
   (h : ∀ c, is_defined x c) :
   Evalable.eval ctx (contract x) = part.some (contract_stream ((Evalable.eval ctx x).get ⟨hctx, h⟩)) :=
 by { rw ← part.get_eq_iff_eq_some, swap, { simp [contract, h, hctx], }, refl, }
+
+lemma contract_spec' [Evalable ι ι'] [Evalable α β] {ctx : EContext} (x : BoundedStreamGen ι α) 
+  (hctx : x.ctx_inv ctx) (motive : StreamExec EContext unit β → Prop)
+  (hyp : ∃ c, c ∈ Evalable.eval ctx x ∧ motive (contract_stream c)) :
+  ∃ c, c ∈ Evalable.eval ctx (contract x) ∧ motive c := sorry
 
 section sparse_vectors
 open NameSpace (reserved) Vars (ind₀ vals len)
@@ -634,6 +640,28 @@ lemma externSparseVec_has_tr (scratch : NameSpace) (c : EContext) :
 lemma externSparseVec_is_defined (scratch : NameSpace) (c : EContext) :
   is_defined (externSparseVec scratch) c := (externSparseVec_has_tr scratch c).is_def
 
+-- set_option pp.all true
+
+lemma externSparseVec_spec (scratch : NameSpace) (c : EContext)
+  (hc : (externSparseVec scratch).ctx_inv c) :
+  ∃ c' : StreamExec EContext ℕ R, c' ∈ Evalable.eval c (externSparseVec scratch) ∧ 
+  c'.eval = 
+  (list.map₂ (λ i x, finsupp.single i x) (c.heap.get (NameSpace.reserved∷Vars.ind₀ : Ident nn)) 
+    (c.heap.get (NameSpace.reserved∷Vars.vals : Ident rr))).sum :=
+begin
+  -- have : (Evalable.eval c (externSparseVec scratch)).dom := ⟨hc, externSparseVec_is_defined scratch⟩,
+  -- rw part.dom_iff_mem at this, cases this with c' hc', refine ⟨c', hc', _⟩,
+  have := @tr_to.eval_finsupp_eq (Expr nn) (Expr rr) ℕ R ℕ _ _ (externSparseVec scratch)
+    (primitives.externSparseVec 
+    (c.heap.get (NameSpace.reserved∷Vars.ind₀ : Ident nn))
+    (c.heap.get (NameSpace.reserved∷Vars.vals : Ident rr)))
+    (λ ctx, ctx.store.get (scratch∷Vars.i : Ident nn)) c _
+    _,
+  swap, { intro ctx,  }
+end
+
+#check @tr_to.eval_finsupp_eq
+
 end sparse_vectors
 
 def compile_scalar (x : BoundedStreamGen unit (Expr rr)) : Prog :=
@@ -643,32 +671,39 @@ Prog.loop x.bound x.valid $
   Prog.branch x.ready (out ::= out + x.value) Prog.skip <;>
   x.next
 
+lemma compile_scalar_sound (x : BoundedStreamGen unit (Expr rr)) (ctx : EContext)
+  (hctx : x.ctx_inv ctx) (h : ∀ c, is_defined x c) :
+  ∃ (c' : EContext), 
+    (compile_scalar x).eval ctx = some c' ∧
+    c'.store.get (NameSpace.reserved∷Vars.output : Ident rr) = ((Evalable.eval ctx x).get ⟨hctx, h⟩).eval () :=
+begin
+  simp [compile_scalar, Prog.eval],
+  sorry,
+end
+
+end stream
+
+end compiler
+
+section examples
+parameters [add_comm_monoid R] [has_one R] [has_mul R]
+
+def sum_vec (scratch : NameSpace) : BoundedStreamGen unit (Expr rr) :=
+contract (externSparseVec scratch)
+
+lemma sum_vec_spec (scratch : NameSpace) (ctx : EContext) (hctx : (externSparseVec scratch).ctx_inv ctx) :
+  ∃ (s : StreamExec EContext unit R), s ∈ Evalable.eval ctx (sum_vec scratch) ∧
+  s.eval () = (ctx.heap.get (NameSpace.reserved∷Vars.vals : Ident rr)).sum :=
+begin
+  apply contract_spec' _ hctx,
+end
+
+end examples
+
+
 -- Final theorem will be something like:
 -- ∀ (x : BoundedStreamGen ι α) [Evalable ι → ι'] [Evalable α → β] [FinsuppEval (StreamExec EContext ι' β)]
 --  (hind₁ : ι compiles correctly) (hind₂ : α compiles correctly) : BoundedStreamGen ι α compiles correctly
-
-
--- structure tr {ι ι' σ α β} (x : BoundedStreamGen ι α) (y : Stream σ ι' β) :=
--- (tr_ι : EContext → ι → ι')
--- (tr_α : EContext → α → β)
--- (tr_ctx : EContext → σ)
--- -- (hcurr : ∀ ctx : EContext, y.stream.valid (tr_ctx ctx) = tt → )
--- (hvalid : ∀ ctx : EContext, ∃ n : ℕ, n ∈ x.valid.eval ctx ∧ (0 < n ↔ y.valid (tr_ctx ctx) = tt))
--- (hready : ∀ ctx : EContext, ∃ n : ℕ, n ∈ x.ready.eval ctx ∧ (0 < n ↔ y.ready (tr_ctx ctx) = tt))
--- (hnext : ∀ ctx : EContext, ∃ ctx' ∈ x.next.eval ctx, y.next (tr_ctx ctx) = tr_ctx ctx')
--- (hval : ∀ ctx : EContext, ∃ n : ℕ, )
--- etc. ℕ
-
-
-
--- (N : Expr nn)
--- tr (range_nn N) (range ?)
-
--- range_nn (n : Expr nn) ∼ range_nn
--- singleton (range_nn (n : Expr nn))  ∼ singleton (range )
-
-
-end stream
 
 
 end
@@ -681,774 +716,9 @@ notation ` Σ_c ` := contract
 def R := ℤ
 abbreviation compile := @compile_scalar R
 
-def sum_vec : BoundedStreamGen R unit (Expr R rr) :=
+def sum_vec' : BoundedStreamGen R unit (Expr R rr) :=
 Σ_c (externSparseVec (fresh ∅))
 
-#eval do io.print_ln (compile sum_vec)
+#eval do io.print_ln (compile sum_vec')
 
 end examples
-
-#exit
-
-@[simp]
-def add : ExprVal → ExprVal → ExprVal
-| (nat n₁) (nat n₂) := nat (n₁ + n₂)
-| (rval f₁) (rval f₂) := rval (f₁ + f₂)
-| _ _ := arbitrary _
-
-@[simp]
-def and : ExprVal → ExprVal → ExprVal
-| (nat n₁) (nat n₂) := if n₁ = 0 then nat 0 else nat n₂
-| _ _ := arbitrary _
-
-@[simp]
-def mul : ExprVal → ExprVal → ExprVal
-| (nat n₁) (nat n₂) := nat (n₁ * n₂)
-| (rval f₁) (rval f₂) := rval (f₁ * f₂)
-| _ _ := arbitrary _
-
-@[simp]
-def not : ExprVal → ExprVal
-| (nat n₁) := if n₁ = 0 then nat 1 else nat 0
-| _ := arbitrary _
-
-@[simp]
-def to_nat : ExprVal → ℕ
-| (nat n₁) := n₁
-| _ := arbitrary _
-
-@[simp]
-def eq : ExprVal → ExprVal → ExprVal
-| (nat n₁) (nat n₂) := if n₁ = n₂ then nat 1 else nat 0
-| _ _ := arbitrary _
-
-@[simp]
-def lt : ExprVal → ExprVal → ExprVal
-| (nat n₁) (nat n₂) := if n₁ < n₂ then nat 1 else nat 0
-| _ _ := arbitrary _
-
-@[simp]
-def to_r : ExprVal → R
-| (nat n) := n
-| (rval r) := r
-
-@[simp]
-def cast_r (v : ExprVal) : ExprVal := rval v.to_r
-
-end ExprVal
-parameter (R)
-inductive IdentVal
-| base (val : ExprVal) : IdentVal
-| arr (val : list (ExprVal)) : IdentVal
-instance : inhabited IdentVal := ⟨IdentVal.base default⟩
-
-parameter {R}
-def IdentVal.get : IdentVal → option ℕ → ExprVal
-| (IdentVal.base val) none := val
-| (IdentVal.arr val) (some i) := val.inth i
-| _ _ := arbitrary _
-
-@[simp] lemma IdentVal.get_none (b : ExprVal) : (IdentVal.base b).get none = b := rfl
-@[simp] lemma IdentVal.get_ind (arr : list ExprVal) (n : ℕ) :
-  (IdentVal.arr arr).get (some n) = arr.inth n := rfl
-
-def IdentVal.update : IdentVal → option ℕ → ExprVal → IdentVal
-| (IdentVal.arr val) (some i) newval := IdentVal.arr (val.modify_nth (λ _, newval) i)
-| _ none newval := IdentVal.base newval
-| _ _ _ := arbitrary _
-
-@[simp] lemma IdentVal.update_none (i : IdentVal) (x : ExprVal) :
-  i.update none x = IdentVal.base x := by cases i; simp [IdentVal.update]
-@[simp] lemma IdentVal.update_ind (arr : list ExprVal) (n : ℕ) (x : ExprVal) :
-  (IdentVal.arr arr).update (some n) x = IdentVal.arr (arr.modify_nth (λ _, x) n) := rfl
-
-end Ident
-
-
-inductive Op
-| add | mul | and | or | not | eq | lt | cast_r
-
-namespace Op
-instance : has_to_string Op := ⟨λ v, match v with
-| add := "add"
-| mul := "mul"
-| and := "and"
-| or := "or"
-| not := "not"
-| eq := "eq"
-| lt := "lt"
-| cast_r := "cast"
-end⟩
-
-@[reducible] def arity : Op → ℕ
-| Op.add := 2
-| Op.mul := 2
-| Op.and := 2
-| Op.or := 2
-| Op.not := 1
-| Op.eq := 2
-| Op.lt := 2
-| Op.cast_r := 1
-
-@[simp]
-def eval : ∀ o : Op, (fin o.arity → ExprVal) → ExprVal
-| add := λ x, (x 0).add (x 1)
-| mul := λ x, (x 0).mul (x 1)
-| and := λ x, (x 0).and (x 1)
-| or := λ x, ((x 0).not.and $ (x 1).not).not -- TODO
-| not := λ x, (x 0).not
-| eq := λ x, (x 0).eq (x 1)
-| lt := λ x, (x 0).lt (x 1)
-| cast_r := λ x, (x 0).cast_r
-end Op
-
-parameter (R)
-inductive Expr
-| lit : ExprVal → Expr
-| ident : Ident → Expr
-| access : Ident → Expr → Expr
-| call : ∀ o : Op, (fin o.arity → Expr) → Expr
-
-parameter {R}
-local notation a ` ⟪+⟫ `:80 b := Expr.call Op.add ![a, b]
-local notation a ` ⟪*⟫ `:80 b := Expr.call Op.mul ![a, b]
-local notation a ` ⟪&&⟫ `:80 b := Expr.call Op.and ![a, b]
-local notation a ` ⟪||⟫ `:80 b := Expr.call Op.or ![a, b]
-local notation a ` ⟪<⟫ `:80 b := Expr.call Op.lt ![a, b]
-local notation a ` ⟪=⟫ `:80 b := Expr.call Op.eq ![a, b]
-
-@[simp]
-def Expr.eval  (ctx : Ident → IdentVal) : Expr → ExprVal
-| (Expr.lit r) := r
-| (Expr.ident x) := (ctx x).get none
-| (Expr.access x i) := (ctx x).get (some i.eval.to_nat)
-| (Expr.call o args) := o.eval (λ i, (args i).eval)
-
-instance has_coe_from_nat : has_coe ℕ Expr := ⟨λ n, Expr.lit $ ExprVal.nat n⟩
-instance has_coe_from_R : has_coe R Expr := ⟨λ r, Expr.lit $ ExprVal.rval r⟩
-instance has_coe_from_Ident : has_coe Ident Expr := ⟨Expr.ident⟩
-
-example : Expr := (0 : ℕ)
-example : Expr := (0 : R)
-
-@[simp] lemma Expr.eval_const_nat (ctx : Ident → IdentVal) (n : ℕ) :
-  Expr.eval ctx n = ExprVal.nat n := rfl
-
-@[simp] lemma Expr.eval_const_r (ctx : Ident → IdentVal) (r : R) :
-  Expr.eval ctx r = ExprVal.rval r := rfl
-
-@[simp] lemma Expr.eval_coe_ident (ctx : Ident → IdentVal) (i : Ident) :
-  Expr.eval ctx i = (ctx i).get none := rfl
-
-/-- Pretty print repr of indices; ignores [] (scalar), represents only
-    vector indices -/
--- def idcs_repr (idcs : list string) : string :=
--- if idcs.length = 0 then "" else "[" ++ ", ".intercalate idcs ++ "]"
-
-def expr_repr [has_to_string R] : Expr → string
-| (Expr.lit r) := to_string r
-| (Expr.ident x) := to_string x
-| (Expr.access x i) := (to_string x) ++ "[" ++ (expr_repr i) ++ "]"
-| (Expr.call o args) := (to_string o) ++ "(" ++ ", ".intercalate (vector.of_fn (λ i, expr_repr $ args i)).to_list ++ ")"
-
-instance [has_to_string R] : has_to_string Expr := ⟨expr_repr⟩
--- Because ambiguous whether R or ℕ
--- instance : has_zero (Expr R) := ⟨Expr.lit 0⟩
--- instance : has_one (Expr R) := ⟨Expr.lit 1⟩
-
-parameter (R)
-structure LoopBound :=
-(frame : finset Ident)
-(to_fun : (Ident → IdentVal) → ℕ)
-(has_frame : function.has_frame to_fun frame)
-
-parameter {R}
-instance : has_coe_to_fun LoopBound (λ _, (Ident → IdentVal) → ℕ) :=
-⟨LoopBound.to_fun⟩
-
-@[simp] lemma to_fun_eq_coe (f : LoopBound) (ctx : Ident → IdentVal) : f.to_fun = ⇑f := rfl
-
-@[simp] lemma to_fun_apply (frame : finset Ident) (to_fun : (Ident → IdentVal) → ℕ) (h) (ctx : Ident → IdentVal) :
-  (LoopBound.mk frame to_fun h) ctx = to_fun ctx := rfl
-
-theorem LoopBound.frame_sound (f : LoopBound) {ctx₀ ctx₁ : Ident → IdentVal} (h : ∀ v ∈ f.frame, ctx₀ v = ctx₁ v) :
-  f ctx₀ = f ctx₁ := function.has_frame_iff.mp f.has_frame h
-
-parameter (R)
-inductive Prog
-| skip : Prog
-| store (dst : Ident) (ind : option Expr) (val : Expr)
-| seq (a : Prog) (b : Prog)
-| branch (cond : Expr) (a : Prog) (b : Prog)
-| loop (n : LoopBound) (b : Prog)
-
-parameter {R}
-def prog_repr [has_to_string R] : Prog → list string
-| Prog.skip := [";"]
-| (Prog.store dst ind val) := [(to_string dst) ++ (ind.elim "" (λ i, "[" ++ to_string i ++ "]")) ++ " := " ++ (to_string val) ++ ";"]
-| (Prog.seq a b) := (prog_repr a) ++ (prog_repr b)
-| (Prog.branch c a b) := ["if " ++ (to_string c)]
-    ++ (prog_repr a).map (λ s, "  " ++ s)
-    ++ ["else"]
-    ++ (prog_repr b).map (λ s, "  " ++ s)
-| (Prog.loop n b) := ["for at most some bounded # of times"]
-    ++ (prog_repr b).map (λ s, "  " ++ s)
-
-instance [has_to_string R] prog_to_string : has_to_string Prog := ⟨λ p, "\n".intercalate (prog_repr p)⟩
-
-
-
-def Prog.eval : Prog → (Ident → IdentVal) → (Ident → IdentVal)
-| Prog.skip ctx := ctx
-| (Prog.store dst ind val) ctx := function.update ctx dst ((ctx dst).update (ind.map (λ i : Expr, (i.eval ctx).to_nat)) (val.eval ctx))
-| (Prog.seq a b) ctx := b.eval (a.eval ctx)
-| (Prog.branch cond a b) ctx := if 0 < (Expr.eval ctx cond).to_nat then a.eval ctx else b.eval ctx
-| (Prog.loop n b) ctx := (nat.iterate b.eval (n ctx)) ctx
-
-def alist.ilookup {α β : Type*} [decidable_eq α] [inhabited β] (s : alist (λ _ : α, β)) (a : α) : β :=
-(s.lookup a).iget
-
--- Faster version of eval
--- TODO: which one should be the "main" one
-def Prog.eval' : Prog → (alist (λ _ : Ident, IdentVal)) → (alist (λ _ : Ident, IdentVal))
-| Prog.skip ctx := ctx
-| (Prog.store dst ind val) ctx := ctx.insert dst ((ctx.ilookup dst).update (ind.map (λ i : Expr, (i.eval ctx.ilookup).to_nat)) (val.eval ctx.ilookup))
-| (Prog.seq a b) ctx := b.eval' (a.eval' ctx)
-| (Prog.branch cond a b) ctx := if 0 < (cond.eval ctx.ilookup).to_nat then a.eval' ctx else b.eval' ctx
-| (Prog.loop n b) ctx := (nat.iterate b.eval' (n ctx.ilookup)) ctx
-
-section frame
-
-@[simp] def Expr.frame : Expr → finset Ident
-| (Expr.lit r) := ∅
-| (Expr.ident i) := {i}
-| (Expr.access x n) := insert x n.frame
-| (Expr.call o args) := finset.bUnion finset.univ (λ i, (args i).frame)
-
-@[simp] lemma Expr_frame_coe_nat (n : ℕ) : (n : Expr).frame = ∅ := rfl
-@[simp] lemma Expr_frame_coe_R (r : R) : (r : Expr).frame = ∅ := rfl
-@[simp] lemma Expr_frame_coe_ident (i : Ident) : (i : Expr).frame = {i} := rfl
-
-
-/-- The evaluation of an Expr depends only on the values in its frame -/
-theorem frame_sound_Expr {e : Expr} {ctx₀ ctx₁ : Ident → IdentVal}
-  (h : ∀ v ∈ e.frame, ctx₀ v = ctx₁ v) : e.eval ctx₀ = e.eval ctx₁ :=
-begin
-  induction e,
-  case Expr.lit : { simp, },
-  case Expr.ident : i { simp [h i _], },
-  case Expr.access : x n ih { simp at h ⊢, specialize ih h.2, simp [ih, h.1], },
-  case Expr.call : o args ih
-  { simp, congr, ext i, apply ih, refine (λ v hv, h v _), simp, refine ⟨_, hv⟩, }
-end
-
-theorem Expr.has_frame (e : Expr) : function.has_frame (λ ctx, e.eval ctx : (Ident → IdentVal) → ExprVal) e.frame :=
-by { rw function.has_frame_iff, intros c₁ c₂, apply frame_sound_Expr, }
-
-@[simp]
-def Prog.frame : Prog → finset Ident
-| Prog.skip := ∅
-| (Prog.store dst none val) := insert dst val.frame
-| (Prog.store dst (some ind) val) := insert dst (ind.frame ∪ val.frame)
-| (Prog.seq a b) := a.frame ∪ b.frame
-| (Prog.branch cond a b) := cond.frame ∪ a.frame ∪ b.frame
-| (Prog.loop n b) := n.frame ∪ b.frame
-
-/-- Ident's not in the frame remain unchanged -/
-theorem not_mem_Prog_frame {p : Prog} {s} (hs : s ∉ p.frame) (ctx : Ident → IdentVal) :
-  p.eval ctx s = ctx s :=
-begin
-  induction p generalizing ctx,
-  case Prog.skip : { simp [Prog.eval], },
-  case Prog.store : dst ind val
-  { suffices : s ≠ dst, { simp [Prog.eval, this] },
-    rintro rfl, cases ind; simpa using hs, },
-  case Prog.seq : a b ih₁ ih₂
-  { simp [decidable.not_or_iff_and_not] at hs,
-    simp [Prog.eval, ih₂ hs.2, ih₁ hs.1], },
-  case Prog.branch : cond a b ih₁ ih₂
-  { simp [decidable.not_or_iff_and_not] at hs,
-    simp [Prog.eval], split_ifs, exacts [ih₁ hs.2.1 _, ih₂ hs.2.2 _], },
-  case Prog.loop : n b ih
-  { simp [Prog.eval],
-    generalize : n ctx = n',
-    induction n' with n' ihn', { refl, },
-    simp [function.iterate_succ_apply'],
-    rwa ih, simp [decidable.not_or_iff_and_not] at hs, exact hs.2, }
-end
-
-/-- If two contexts agree on a set S ⊇ p.frame, then they agree after the evaluation as well. -/
-theorem frame_sound_Prog {p : Prog} {ctx₀ ctx₁ : Ident → IdentVal} {S : finset Ident} (hS : p.frame ⊆ S)
-  (h : ∀ v ∈ S, ctx₀ v = ctx₁ v) {s} (hs : s ∈ S) : p.eval ctx₀ s = p.eval ctx₁ s :=
-begin
-  induction p generalizing ctx₀ ctx₁ s,
-  case Prog.skip : { simpa [Prog.eval] using h _ hs, },
-  case Prog.store : dst ind val
-  { by_cases s_eq : s = dst, swap, { simpa [Prog.eval, s_eq] using h _ hs, },
-    subst s_eq, simp [Prog.eval], congr' 1, { exact h _ hs, },
-    { cases ind; simp, congr' 1, apply frame_sound_Expr, refine λ v hv, h v _, simp [finset.subset_iff] at hS, apply hS.2, left, exact hv, },
-    apply frame_sound_Expr, refine λ v hv, h v _, cases ind; simp [finset.subset_iff] at hS, exacts [hS.2 _ hv, hS.2 _ (or.inr hv)], },
-  case Prog.seq : a b ih₁ ih₂
-  { simp [Prog.eval],
-    simp at hS, refine ih₂ (finset.union_subset_right hS) _ hs,
-    intros v hv, exact ih₁ (finset.union_subset_left hS) h hv, },
-  case Prog.branch : cond a b ih₁ ih₂
-  { have : cond.eval ctx₀ = cond.eval ctx₁,
-    { apply frame_sound_Expr, refine λ v hv, h v _,
-      simp [finset.subset_iff] at hS, exact hS (or.inl hv), },
-    simp [Prog.eval, this], simp at hS, split_ifs,
-    { exact ih₁ (finset.union_subset_left (finset.union_subset_right hS)) h hs, },
-    exact ih₂ (finset.union_subset_right (finset.union_subset_right hS)) h hs, },
-  case Prog.loop : n b ih
-  { have : n ctx₀ = n ctx₁,
-    { apply LoopBound.frame_sound, refine λ v hv, h v _, simp [finset.subset_iff] at hS, exact hS (or.inl hv), },
-    simp [Prog.eval, this],
-    generalize : n ctx₁ = n',
-    induction n' with n' ihn generalizing s, { exact h _ hs, },
-    simp [function.iterate_succ_apply'],
-    refine ih _ @ihn hs, simp at hS, exact finset.union_subset_right hS, }
-end
-
-def Expr.to_loop_bound (e : Expr) : LoopBound :=
-{ frame := e.frame,
-  to_fun := λ ctx, (e.eval ctx).to_nat,
-  has_frame := (Expr.has_frame e).postcomp _ }
-
-@[simp] lemma Expr.to_loop_bound_to_fun (e : Expr) (ctx : Ident → IdentVal) : e.to_loop_bound ctx = (e.eval ctx).to_nat :=
-by simp [Expr.to_loop_bound]
-
-
-end frame
-
-local infixr ` <;> `:1 := Prog.seq
-local notation a ` ::= `:20 c := Prog.store a none c
-local notation a ` ⟬ `:9000 i ` ⟭ ` ` ::= `:20 c := Prog.store a (some i) c
-local notation x ` ⟬ `:9000 i ` ⟭ ` := Expr.access x i
-
-parameter (R)
-structure BoundedStreamGen (ι α : Type) :=
-(current : ι)
-(value : α)
-(ready : Expr)
-(next : Prog)
-(valid : Expr)
-(bound : LoopBound)
-(initialize : Prog)
-
-parameter {R}
-@[ext]
-theorem BoundedStreamGen.ext {ι α} {x y : BoundedStreamGen ι α} (h₀ : x.current = y.current)
-  (h₁ : x.value = y.value) (h₂ : x.ready = y.ready) (h₃ : x.next = y.next) (h₄ : x.valid = y.valid)
-  (h₅ : x.bound = y.bound) (h₆ : x.initialize = y.initialize) : x = y :=
-by { cases x, cases y, dsimp only at *, subst_vars, }
-
-variables {ι α : Type}
-
-section functorality
-
-@[simps]
-instance : bifunctor BoundedStreamGen :=
-{ bimap := λ _ _ _ _ i v g, { g with value := v g.value, current := i g.current } }
-
-instance : is_lawful_bifunctor BoundedStreamGen :=
-{ id_bimap := λ _ _ g, by ext; simp [bimap],
-  bimap_bimap := λ _ _ _ _ _ _ i i' v v' g, by ext; simp [bimap] }
-
-infixr ` <$₁> `:1 := bifunctor.fst
-infixr ` <$₂> `:1 := bifunctor.snd
-
--- TODO: find a better way
-variables {ι' α' : Type} (f : ι → ι') (g : α → α') (s : BoundedStreamGen ι α)
-@[simp] lemma BSG_fst_value : (f <$₁> s).value = s.value := rfl
-@[simp] lemma BSG_fst_ready : (f <$₁> s).ready = s.ready := rfl
-@[simp] lemma BSG_fst_next : (f <$₁> s).next = s.next := rfl
-@[simp] lemma BSG_fst_valid : (f <$₁> s).valid = s.valid := rfl
-@[simp] lemma BSG_fst_bound : (f <$₁> s).bound = s.bound := rfl
-@[simp] lemma BSG_fst_init : (f <$₁> s).initialize = s.initialize := rfl
-@[simp] lemma BSG_snd_current : (g <$₂> s).current = s.current := rfl
-@[simp] lemma BSG_snd_ready : (g <$₂> s).ready = s.ready := rfl
-@[simp] lemma BSG_snd_next : (g <$₂> s).next = s.next := rfl
-@[simp] lemma BSG_snd_valid : (g <$₂> s).valid = s.valid := rfl
-@[simp] lemma BSG_snd_bound : (g <$₂> s).bound = s.bound := rfl
-@[simp] lemma BSG_snd_init : (g <$₂> s).initialize = s.initialize := rfl
-
-@[simp] lemma BSG_fst_current : (f <$₁> s).current = f s.current := rfl
-@[simp] lemma BSG_snd_value : (g <$₂> s).value = g s.value := rfl
-
-attribute [functor_norm] bifunctor.fst_snd bifunctor.snd_fst
-
-end functorality
-
-@[pattern]
-def Prog.if1 (cond : Expr) (b : Prog) := Prog.branch cond b Prog.skip
-
-def BoundedStreamGen.compile (g : BoundedStreamGen unit Prog) : Prog :=
-g.initialize <;>
-Ident.mk default Vars.break ::= (0 : ℕ) <;>
-Prog.loop g.bound $
-  Prog.if1 (Expr.call Op.not ![Ident.mk default Vars.break]) $
-    Prog.if1 g.ready g.value <;>
-    Prog.branch g.valid g.next (Ident.mk default Vars.break ::= (1 : ℕ))
-
-parameter (R)
-/-- Indicates that things of type α (which typically involve Expr R)'s can eval
-  to things of type β given a context ctx : Ident → IdentVal R -/
-class StreamEval (α β: Type) :=
-(eval : α → (Ident → IdentVal) → β)
-
-/-- An Compileable.compile (f, e) indicates that f describes how to compile e to a program -/
-class Compileable (α β : Type) :=
-(compile : α → β → Prog)
-
-parameter {R}
--- This is ind_eval, but we need to support recursion so we extract it specifically
--- Mathlib's lack of computability bites here;
--- since finsupp is noncomputable (this is actually a controversial-ish decision from what I gather from the Zulip)
--- it poisons "eval_stream"
--- We only use +, finsupp.single and finsupp.zero (zero is computable), so maybe a TODO is a computable implementation
-@[simp]
-noncomputable def eval_stream {ι β : Type} [add_zero_class β] :
-  ℕ → (Ident → IdentVal) → (BoundedStreamGen ((Ident → IdentVal) → ι) ((Ident → IdentVal) → β)) → (ι →₀ β)
-| 0 _ _ := 0
-| (n+1) ctx s :=
-if (s.valid.eval ctx).to_nat = 1 then
-  (if (s.ready.eval ctx).to_nat = 1 then finsupp.single (s.current ctx) (s.value ctx) else 0)
-    + (eval_stream n (s.next.eval ctx) s)
-else 0
-
-instance base_eval : StreamEval Expr ExprVal :=
-⟨λ e ctx, e.eval ctx⟩
-
-instance base_eval_nat : StreamEval Expr ℕ :=
-⟨λ e ctx, (e.eval ctx).to_nat⟩
-
-instance base_eval_R : StreamEval Expr R :=
-⟨λ e ctx, (e.eval ctx).to_r⟩
-
-instance refl_eval {α : Type} : StreamEval α α := ⟨λ x _, x⟩
-
-noncomputable instance ind_eval {ι ι' α β : Type} [StreamEval ι ι'] [StreamEval α β] [add_zero_class β] :
-  StreamEval (BoundedStreamGen ι α) (ι' →₀ β) :=
-{ eval := λ s ctx, eval_stream (s.bound ctx) (s.initialize.eval ctx)
-  (StreamEval.eval <$₁> StreamEval.eval <$₂> s) }
-
-/- Convenience instance for `unit` so we don't have to write `unit → R` and can directly go to R
-TODO: Remove? -/
-noncomputable instance unit_eval {α β : Type} [StreamEval α β] [add_zero_class β] :
-  StreamEval (BoundedStreamGen unit α) β :=
-{ eval := λ s ctx, (StreamEval.eval s ctx : unit →₀ β) () }
-
-instance base_compile : Compileable (Expr → Prog) Expr :=
-⟨λ c e, c e⟩
-
-section laws
--- Law 1: eval frame should be frame
-structure BoundedStreamGen.has_frame (x : BoundedStreamGen ι α) (ι' β) [StreamEval ι ι'] [StreamEval α β] (S : set Ident) :=
-(current : function.has_frame (StreamEval.eval x.current : _ → ι') S)
-(value : function.has_frame (StreamEval.eval x.value : _ → β) S)
-(ready : ↑x.ready.frame ⊆ S)
-(next : ↑x.next.frame ⊆ S)
-(valid : ↑x.valid.frame ⊆ S)
-(bound : ↑x.bound.frame ⊆ S)
-(initialize : ↑x.initialize.frame ⊆ S)
-
-theorem eval_has_frame_of_has_frame {ι' β S} [StreamEval ι ι'] [StreamEval α β] [add_zero_class β] {x : BoundedStreamGen ι α} (hx : x.has_frame ι' β S) :
-  function.has_frame (StreamEval.eval x : _ → (ι' →₀ β)) S :=
-begin
-  sorry,
-end
-
-
--- Law 2: eval for bound steps should make invalid
-
-end laws
-
-section variable_state
-
-structure WithFrame (α : Type) : Type :=
-(val : α)
-(frame : finset NameSpace)
-
-instance WithFrame_coe {α : Type} : has_coe (WithFrame α) α := ⟨WithFrame.val⟩
-
-@[simp] lemma WithFrame_coe_val (x : WithFrame α) : x.val = (x : α) := rfl
-
-@[simp] lemma WithFrame.val_eq (val : α) (frame : finset NameSpace) :
-  (WithFrame.mk val frame : α) = val := rfl
-
-@[simp] lemma WithFrame.frame_eq (val : α) (frame : finset NameSpace) :
-  (WithFrame.mk val frame).frame = frame := rfl
-
-parameter (R)
-def WithFrame.is_sound (x : WithFrame α) (β : Type) [StreamEval α β] : Prop :=
-function.has_frame (StreamEval.eval (x : α) : (Ident → IdentVal) → β) (Ident.ns⁻¹' x.frame)
-
-parameter {R}
-def WithFrame.fresh {β : Type} (x : finset NameSpace) (f : NameSpace → β) : WithFrame β :=
-⟨f (fresh x), insert (fresh x) x⟩
-
-lemma WithFrame.fresh_spec (x : finset NameSpace) ⦃v : Ident⦄ (hx : v.ns ∈ x) (v' : Vars) :
-  v ≠ (fresh x)∷v' :=
-by { rintro rfl, exact not_fresh_mem _ hx, }
-
-lemma WithFrame.is_sound_of_fresh₁ {ι' β} [add_zero_class β] [StreamEval ι ι'] [StreamEval α β] (x : finset NameSpace) {f : NameSpace → BoundedStreamGen ι α}
-  (hf : BoundedStreamGen.has_frame (f (fresh x)) ι β (Ident.ns⁻¹' (insert (fresh x) x))) :
-  WithFrame.is_sound (WithFrame.fresh x f) (ι →₀ β) :=
-begin
-  simp [WithFrame.is_sound], sorry,
-end
-
-lemma WithFrame.is_sound_of_fresh₂ {β} [add_zero_class β] [StreamEval α β] (x : finset NameSpace) {f : NameSpace → (BoundedStreamGen unit α)}
-  (hf : BoundedStreamGen.has_frame (f (fresh x)) unit β (Ident.ns⁻¹' (insert (fresh x) x))) :
-  WithFrame.is_sound (WithFrame.fresh x f) β :=
-begin
-  simp [WithFrame.is_sound], sorry,
-end
-
-
--- (current : ι)
--- (value : α)
--- (ready : Expr)
--- (next : Prog)
--- (valid : Expr)
--- (bound : Expr)
--- (initialize : Prog)
-
-end variable_state
--- example (i : Ident) :  := rfl
-
-section singleton
-open Vars (i)
-
-def BoundedStreamGen.singleton (a : WithFrame α) : WithFrame (BoundedStreamGen unit α) :=
-WithFrame.fresh a.frame $ λ ns,
-{ current := (),
-  value := a,
-  ready := (1 : ℕ),
-  valid := ns∷i ⟪<⟫ (1 : ℕ),
-  bound := ⟨∅, λ _, 1, function.has_frame.const _ _ _⟩,
-  next := ns∷i ::= (1 : ℕ),
-  initialize := ns∷i ::= (0 : ℕ) }
-
-theorem singleton_spec {β : Type} [add_zero_class β] [StreamEval α β] (ctx : Ident → IdentVal) (a : WithFrame α)
-  (h : WithFrame.is_sound a β) :
-  (StreamEval.eval (BoundedStreamGen.singleton a).val ctx : β) = StreamEval.eval a.val ctx :=
-begin
-  simp only [BoundedStreamGen.singleton, WithFrame.fresh],
-  have := WithFrame.fresh_spec a.frame, set ns := fresh a.frame,
-  simp [StreamEval.eval, Prog.eval], rw [WithFrame.is_sound, function.has_frame_iff] at h,
-  apply h, intros x hx, simp [this hx],
-end
-
-theorem singleton_frame_sound {β : Type} [add_zero_class β] [StreamEval α β] {a : WithFrame α}
-  (h : WithFrame.is_sound a β) : WithFrame.is_sound (BoundedStreamGen.singleton a) β :=
-begin
-  simp only [BoundedStreamGen.singleton], apply WithFrame.is_sound_of_fresh₂,
-  split,
-  { simp [StreamEval.eval], apply function.has_frame.mono, apply function.has_frame.const, exact set.empty_subset _, },
-  { simp, apply function.has_frame.mono, exact h, simp [set.preimage_subset_preimage_iff], },
-  all_goals { simp [fin.forall_fin_two], },
-end
-
-end singleton
-
-
-
-def BoundedStreamGen.expr_to_prog (inp : BoundedStreamGen unit Expr) : BoundedStreamGen unit Prog :=
-{ current := (),
-  value := NameSpace.reserved∷Vars.output ::= NameSpace.reserved∷Vars.output ⟪+⟫ inp.value,
-  ready := inp.ready,
-  next := inp.next,
-  valid := inp.valid,
-  bound := inp.bound,
-  initialize := inp.initialize <;> NameSpace.reserved∷Vars.output ::= (0 : R) }
-
--- section example_singleton
-
--- def test : BoundedStreamGen ℤ unit (Expr ℤ) := M.get (BoundedStreamGen.singleton (10 : ℤ))
-
--- lemma test_eval : (StreamEval.eval (λ _, arbitrary (IdentVal ℤ)) test : ℤ) = 10 :=
--- by { simp [StreamEval.eval, test, Prog.eval, BoundedStreamGen.singleton], }
-
--- end example_singleton
-
-section range
-
-def range_aux (n : Expr) (v : Ident) : BoundedStreamGen Expr Expr :=
-{ current := v,
-  value := Expr.call Op.cast_r ![v],
-  ready := (1 : ℕ),
-  valid := v ⟪<⟫ n,
-  next := v ::= v ⟪+⟫ (1 : ℕ),
-  bound := (n : Expr).to_loop_bound,
-  initialize := v ::= (0 : ℕ), }
-
-def range (n : WithFrame Expr) : WithFrame (BoundedStreamGen Expr Expr) :=
-WithFrame.fresh n.frame $ λ ns, range_aux n ns∷Vars.i
-
-lemma range_spec_aux (bound n x₀ : ℕ) (hn : n ≤ x₀ + bound)
-  (ctx : Ident → IdentVal)
-  (n' : WithFrame Expr) (hn' : Expr.eval ctx n' = ExprVal.nat n)
-  (n'_sound : WithFrame.is_sound n' ExprVal)
-  (v : Ident) (hv : v.ns ∉ n'.frame) (hx₀ : ctx v = IdentVal.base (ExprVal.nat x₀)) :
-  ∀ (t : ℕ), eval_stream bound ctx ((λ (e : Expr) ctx, (e.eval ctx).to_nat) <$₁> (λ (e : Expr) ctx, (e.eval ctx).to_r) <$₂> (range_aux n' v)) t =
-   (if x₀ ≤ t ∧ t < n then (t : R) else 0) :=
-begin
-  induction bound with bound ih generalizing ctx x₀,
-  { intro t, simp, split_ifs, { cases not_lt.mpr (hn.trans h.1) h.2, }, refl, },
-  intro t, simp [range_aux, hx₀, hn', ← apply_ite _root_.ExprVal.nat, imp_false],
-  by_cases h : x₀ < n, swap,
-  { have h' : ¬(x₀ ≤ t ∧ t < n) := λ H, h (lt_of_le_of_lt H.1 H.2), simp [h, h'], },
-  simp [h, Prog.eval, hx₀],
-  rw [← range_aux, ih (function.update ctx v (IdentVal.base (ExprVal.nat $ x₀ + 1))) (x₀ + 1) _ _ _]; clear ih,
-  { by_cases H : x₀ = t, { subst H, simp [h], }, simp [ne.le_iff_lt H, ← nat.succ_le_iff, H, nat.succ_eq_add_one], },
-  { refine hn.trans (le_of_eq _), rw nat.succ_eq_add_one, ac_refl, },
-  { simp only [WithFrame.is_sound, function.has_frame_iff, StreamEval.eval] at n'_sound, rw ← hn', apply n'_sound,
-    simp_intros x hx, suffices : x ≠ v, { simp [this], }, rintro rfl, exact hv hx, },
-  { simp, }
-end
-
-example (a b :ℕ) (h : a ≠ b) : a + 1 ≤ b ↔ a ≤ b :=
-by { rw nat.succ_le_iff, exact (ne.le_iff_lt h).symm}
-
-theorem range_spec (n : WithFrame Expr) (hn : WithFrame.is_sound n ExprVal) (ctx : Ident → IdentVal) (n' : ℕ)
-  (hn' : Expr.eval ctx n = ExprVal.nat n') :
-  (StreamEval.eval (range n).val ctx : ℕ →₀ R) = finsupp.indicator (finset.range n') (λ i _, (i : R)) :=
-begin
-  simp only [StreamEval.eval, range, WithFrame.fresh],
-  have n_fresh := WithFrame.fresh_spec n.frame, set ns := fresh n.frame,
-  ext t,
-  convert range_spec_aux ((n : Expr).to_loop_bound ctx) n' 0 _ ((range_aux n ns∷Vars.i).initialize.eval ctx) n _ hn ns∷Vars.i _ _ t, { simp, },
-  { simp [hn'], },
-  { simp only [WithFrame.is_sound, function.has_frame_iff, StreamEval.eval] at hn, rw ← hn', apply hn, simp_intros x hx, suffices : x ≠ ns∷Vars.i, { simp [range_aux, Prog.eval, this], }, rintro rfl, exact n_fresh hx _ rfl, },
-  { intro h, exact n_fresh h _ rfl, },
-  { simp [range_aux, Prog.eval], },
-end
-
-end range
-
-section contract
-
-def contract (g : BoundedStreamGen ι α) : BoundedStreamGen unit α :=
-(λ _, ()) <$₁> g
-
-lemma contract_aux [add_comm_monoid α] (n : ℕ) (ctx : Ident → IdentVal)
-  (g : BoundedStreamGen ((Ident → IdentVal) → ι) ((Ident → IdentVal) → α)) :
-  (eval_stream n ctx ((λ _ _, ()) <$₁> g)) () = (eval_stream n ctx g).sum_range :=
-begin
-  induction n with n ih generalizing ctx, { simp, },
-  simp,
-  split_ifs,
-  { simp [← ih (g.next.eval ctx)], }, -- Valid and ready
-  { simp [← ih (g.next.eval ctx)], }, -- Valid but not ready
-  refl, -- Invalid, both are 0
-end
-
-theorem contract_spec {β ι' : Type} [add_comm_monoid β] [StreamEval α β] [StreamEval ι ι']
-  (s : BoundedStreamGen ι α) (ctx : Ident → IdentVal) :
-  StreamEval.eval (contract s) ctx = (StreamEval.eval s ctx : ι' →₀ β).sum_range :=
-by simpa [StreamEval.eval, contract, bifunctor.fst] with functor_norm
-using contract_aux (s.bound ctx) (s.initialize.eval ctx)
-      (StreamEval.eval <$₁> StreamEval.eval <$₂> s)
-
-end contract
-
-section repeat
-
-end repeat
-
-def flatten {ι₁ ι₂ α : Type} (outer : BoundedStreamGen ι₁ (BoundedStreamGen ι₂ α)) :
-  BoundedStreamGen (ι₁ × ι₂) α :=
-let inner := outer.value in
-{ current := (outer.current, inner.current),
-  value := inner.value,
-  ready := outer.ready ⟪&&⟫ inner.ready,
-  next := let next_outer := outer.next <;> inner.initialize in
-  Prog.branch outer.ready
-    (Prog.branch inner.valid inner.next next_outer)
-    next_outer,
-  valid := outer.valid,
-  bound := sorry, --outer.bound ⟪*⟫ inner.bound, -- TODO: fix
-  initialize := outer.initialize <;> inner.initialize }
-
--- def test₂ : BoundedStreamGen ℤ (Expr ℤ) (Expr ℤ) := range (40 : ℕ) vars.x
--- #eval trace_val $ to_string $ (contract test₂).expr_to_prog.compile
--- #eval (((contract test₂).expr_to_prog.compile.eval' ∅).ilookup vars.output).get none
-
-def externVec (len : Expr) (inp : Ident) (inp_idx : Ident) : BoundedStreamGen Expr Expr :=
-{ current := inp_idx,
-  value := inp⟬ inp_idx ⟭,
-  ready := inp_idx ⟪<⟫ len,
-  next := inp_idx ::= inp_idx ⟪+⟫ (1 : ℕ),
-  valid := inp_idx ⟪<⟫ len,
-  bound := len.to_loop_bound,
-  initialize := inp_idx ::= (0 : ℕ) }
-
-def externCSRMat (l₁ l₂ : Expr) (rows cols data : Ident) (i j k : Ident) :
-  BoundedStreamGen (Expr × Expr) Expr :=
-{ current := (i, cols⟬j⟭),
-  value := data⟬k⟭,
-  ready := j ⟪<⟫ rows⟬i ⟪+⟫ (1 : ℕ)⟭,
-  next :=
-    k ::= k ⟪+⟫ (1 : ℕ) <;>
-    Prog.branch (j ⟪<⟫ rows⟬i ⟪+⟫ (1 : ℕ)⟭)
-      (j ::= j ⟪+⟫ (1 : ℕ))
-      (i ::= i ⟪+⟫ (1 : ℕ)),
-  valid := i ⟪<⟫ l₁,
-  bound := sorry, --l₁ ⟪*⟫ l₂ ,
-  initialize := i ::= (0 : ℕ) <;> j ::= (0 : ℕ) <;> k ::= (0 : ℕ), }
-
-
--- def test₃ : BoundedStreamGen ℤ (Expr ℤ) (Expr ℤ) := externVec (10 : ℕ) (Ident.of "input") (Ident.of "idx")
-
--- #eval trace_val $ to_string $ (contraction (Ident.of "acc") test₃).expr_to_prog.compile
-
-end
-
--- Examples
-
--- section example_prog
--- namespace vars
-
--- abbreviation x := Ident.of "x"
--- abbreviation y := Ident.of "y"
--- abbreviation z := Ident.of "z"
--- abbreviation s := Ident.of "s"
--- abbreviation i := Ident.of "i"
--- abbreviation acc := Ident.of "acc"
--- abbreviation output := Ident.of "output"
-
--- end vars
-
--- open Expr Prog vars
-
--- def pow_prog : Prog ℤ :=
--- z ::= (1 : ℤ) <;>
--- loop ⟨_, _, function.has_frame.const _ _ 4⟩ (z ::= x ⟪*⟫ z)
-
--- def pow_prog_input (i : Ident) : IdentVal ℤ :=
---   if i = x then IdentVal.base (ExprVal.rval 3)
---   else if i = y then IdentVal.base (ExprVal.nat 4)
---   else arbitrary _
-
--- def arr_prog : Prog ℤ :=
--- s ::= (0 : ℤ) <;>
--- i ::= (0 : ℕ) <;>
--- loop (Expr.to_loop_bound y) $
---   s ::= s ⟪+⟫ x⟬i⟭ <;>
---   i ::= i ⟪+⟫ (1 : ℕ)
-
--- def arr_prog_input (i : Ident) : IdentVal ℤ :=
---   if i = x then IdentVal.arr [ExprVal.rval 30, ExprVal.rval (-1), ExprVal.rval 4]
---   else if i = y then IdentVal.base (ExprVal.nat 3)
---   else arbitrary _
-
--- def range_sum : Prog ℤ :=
--- s ::= (0 : ℤ) <;>
--- i ::= (0 : ℕ) <;>
--- loop ⟨_, _, function.has_frame.const _ _ 500⟩ $
---   s ::= s ⟪+⟫ (Expr.call Op.cast_r ![i]) <;>
---   i ::= i ⟪+⟫ (1 : ℕ)
-
-
--- end example_prog
